build.OSX.jenkins.sh
@@ -14,7 +14,8 @@ sn -k UT/ut.snk
 xbuild /t:clean /p:Configuration="Debug" /p:Platform="${PLATFRM}" eLyKseeR-base.OSX.sln
 xbuild /p:Configuration="Debug" /p:Platform="${PLATFRM}" eLyKseeR-base.OSX.sln
 
-mono packages/NUnit.Runners.lite.2.6.4.20150512/nunit-console.exe -labels UT/bin/Debug/UT.exe
+#mono packages/NUnit.Runners.lite.2.6.4.20150512/nunit-console.exe -labels UT/bin/Debug/UT.exe
+mono packages/NUnit.ConsoleRunner.3.8.0/tools/nunit3-console.exe UT/bin/Debug/UT.exe
 
 # NUnit test results in: TestResult.xml
 
