default.nix
@@ -1,0 +1,21 @@
+with import <nixpkgs> {};
+
+stdenv.mkDerivation rec {
+    name = "env";
+
+    #src = ./.;
+
+    # Customizable development requirements
+    nativeBuildInputs = [
+        cmake
+        git
+    ];
+
+    buildInputs = [
+        openssl
+        zlib
+        boost
+    ];
+
+}
+
