tests/cpp/utLiz.cpp.md
@@ -23,7 +23,7 @@ BOOST_AUTO_TEST_CASE( copyright_message )
 {
 	std::string msg = lxr::Liz::copyright();
 	std::string veritas = "Copyright";
-	// std::clog << std::endl << msg << std::endl;
+	std::clog << std::endl << msg << std::endl;
 	BOOST_CHECK_EQUAL(msg.substr(0,9), veritas);
 }
 ```
@@ -34,7 +34,7 @@ BOOST_AUTO_TEST_CASE( version_message )
 {
 	std::string msg = lxr::Liz::version();
 	std::string veritas = "Version";
-	// std::clog << std::endl << msg << std::endl;
+	std::clog << std::endl << msg << std::endl;
 	BOOST_CHECK_EQUAL(msg.substr(0,7), veritas);
 }
 ```
@@ -45,7 +45,7 @@ BOOST_AUTO_TEST_CASE( license_message )
 {
 	std::string msg = lxr::Liz::license();
 	std::string veritas = "                    GNU GENERAL PUBLIC LICENSE";
-	// std::clog << std::endl << msg << std::endl;
+	std::clog << std::endl << msg << std::endl;
 	BOOST_CHECK_EQUAL(msg.substr(0,46), veritas);
 }
 ```
@@ -56,7 +56,7 @@ BOOST_AUTO_TEST_CASE( name_message )
 {
 	std::string msg = lxr::Liz::name();
 	std::string veritas = "LXR";
-	// std::clog << std::endl << msg << std::endl;
+	std::clog << std::endl << msg << std::endl;
 	BOOST_CHECK_EQUAL(msg.substr(0,3), veritas);
 }
 ```
